revising epoch_footprint_inv to keep the region of the epoch readers and writers disjoint from the region of the handshake state

src/tls/Handshake.fsti
@@ -103,41 +103,44 @@ val processServerHello: c:config -> option ri -> eph_c -> ch -> sh ->
 // relocate?
 type fresh_subregion r0 r h0 h1 = fresh_region r h0 h1 /\ extends r r0
 
-type epoch_region_inv (#i:id) (rgn:rid) (peer:rid) (r:reader (peerId i)) (w:writer i) =
-  parent (region r) = rgn /\ 
-  parent (region w) = rgn /\ 
-  parent (peer_region r) = peer /\
-  disjoint rgn peer /\
-  disjoint (region r) (region w) /\
-  (is_stateful_lhae i ==> 
-    parent (peer_region w) = peer /\
-    disjoint (peer_region r) (peer_region w))
+
+type epoch_region_inv (#i:id) (hs_rgn:rgn) (hs_peer:rgn) (r:reader (peerId i)) (w:writer i) =
+  disjoint hs_rgn hs_peer                     /\ 
+  disjoint hs_rgn (region w)                  /\ 
+  parent (region w) <> FStar.HyperHeap.root    /\
+  parent (region r) <> FStar.HyperHeap.root    /\
+  parent hs_rgn = parent (parent (region w))  /\ //Grandparent of each writer is a sibling of the handshake
+  disjoint hs_peer (region r)                 /\ 
+  parent hs_peer = parent (parent (region r)) /\ //likewise for the peer
+  disjoint (region w) (region r)     
  
-type epoch (rgn:rid) (peer:rid) =
+type epoch (hs_rgn:rgn) (hs_peer:rgn) =
   | Epoch: h: handshake ->
            r: reader (peerId (hsId h)) ->
-           w: writer (hsId h) {epoch_region_inv rgn peer r w} -> epoch rgn peer
+           w: writer (hsId h) {epoch_region_inv hs_rgn hs_peer r w} -> epoch hs_rgn hs_peer
   // we would extend/adapt it for TLS 1.3,
   // e.g. to notify 0RTT/forwad-privacy transitions
   // for now epoch completion is a total function on handshake --- should be stateful
 
 (* The footprint just includes the writer regions *)
-let epochs_footprint (#r:rid) (#p:rid) (es: seq (epoch r p)) =
+let epochs_footprint_inv (#r:rgn) (#p:rgn) (es: seq (epoch r p)) =
   forall (i:nat { i < Seq.length es })
     (j:nat { j < Seq.length es /\ i <> j}).{:pattern (Seq.index es i); (Seq.index es j)}
     let ei = Seq.index es i in
     let ej = Seq.index es j in
-    disjoint (region ei.w) (region ej.w)
+    parent (region ei.w) = parent (region ej.w) /\  //they all descend from a common epochs sub-region of the connection
+    disjoint (region ei.w) (region ej.w)          
  
-let epochs (r:rid) (p:rid) = es: seq (epoch r p) { epochs_footprint es }
+let epochs (r:rgn) (p:rgn) = es: seq (epoch r p) { epochs_footprint_inv es }
 
 // internal stuff: state machine, reader/writer counters, etc.
 // (will take other HS fields as parameters)
 val handshake_state : role -> Type0
+#reset-options "--z3timeout 3 --initial_fuel 2 --max_fuel 2 --initial_ifuel 2 --max_ifuel 2"
 
 type hs =
-  | HS: #region: rid ->
-        #peer: rid ->
+  | HS: #region: rgn ->
+        #peer: rgn ->
         r:role ->
         resume: option (sid:sessionID { r = Client }) ->
         cfg:config ->
@@ -145,6 +148,7 @@ type hs =
         log: rref region (epochs region peer) ->  // append-only; use monotonic? 
         state: rref region (handshake_state r)  ->  // opaque, subject to invariant
         hs
+
 
 (* the handshake internally maintains epoch 
    indexes for the current reader and writer *)
@@ -206,7 +210,7 @@ let latest h (s:hs{Seq.length (sel h s.log) > 0}) = // accessing the latest epoc
 
 
 // placeholder, to be implemented as a stateful property.
-assume val completed: #region:rid -> #peer:rid -> epoch region peer -> Type0
+assume val completed: #region:rgn -> #peer:rgn -> epoch region peer -> Type0
 
 // consider adding an optional (resume: option sid) on the client side
 // for now this bit is not explicitly authenticated.
